[pcm_lens]es compose

pulse/examples/steel/StructRef.fst
@@ -6,15 +6,27 @@ module M = Steel.Memory
 noeq type lens (a: Type u#a) (b: Type u#b) = {
   get: a -> b;
   put: b -> a -> a;
-  get_put: s: a -> v: b -> Lemma (get (put v s) == v);
-  put_get: s: a -> Lemma (put (get s) s == s);
-  put_put: s: a -> v: b -> w: b -> Lemma (put v (put w s) == put v s);
+  get_put: s: a -> v: b -> Lemma (get (put v s) == v); // [SMTPat (get (put v s))];
+  put_get: s: a -> Lemma (put (get s) s == s); // [SMTPat (put (get s) s)];
+  put_put: s: a -> v: b -> w: b -> Lemma (put v (put w s) == put v s); // [SMTPat (put v (put w s))];
 }
+
+let get_put' (l: lens 'a 'b) (s: 'a) (v: 'b)
+  : Lemma (l.get (l.put v s) == v) [SMTPat (l.get (l.put v s))]
+  = l.get_put s v
+
+let put_get' (l: lens 'a 'b) (s: 'a)
+  : Lemma (l.put (l.get s) s == s) [SMTPat (l.put (l.get s))]
+  = l.put_get s
+
+let put_put' (l: lens 'a 'b) (s: 'a) (v w: 'b)
+  : Lemma (l.put v (l.put w s) == l.put v s) [SMTPat (l.put v (l.put w s))]
+  = l.put_put s v w
 
 let upd (l: lens 'a 'b) (f: 'b -> 'b) (s: 'a): 'a = l.put (f (l.get s)) s
 
 (* The non-computational part of frame_preserving_upd *)
-let frame_preserv (p: pcm 'a) (f: 'a -> 'a) (x y: Ghost.erased 'a) =
+let frame_pres (p: pcm 'a) (f: 'a -> 'a) (x y: Ghost.erased 'a) =
   forall (v:'a{p.refine v /\ compatible p x v}).{:pattern compatible p x v}
   p.refine (f v) /\
   compatible p y (f v) /\
@@ -22,25 +34,72 @@ let frame_preserv (p: pcm 'a) (f: 'a -> 'a) (x y: Ghost.erased 'a) =
      composable p y frame /\
      (op p x frame == v ==> op p y frame == f v))
 
-(* Every function satisfying frame_preserv is a frame_preserving_upd *)
-let frame_preserv_mk_upd (p: pcm 'a) (x y: Ghost.erased 'a)
-  (f:('a -> 'a){frame_preserv p f x y})
+(* Every function satisfying frame_pres is a frame_preserving_upd *)
+let frame_pres_mk_upd (p: pcm 'a) (x y: Ghost.erased 'a)
+  (f:('a -> 'a){frame_pres p f x y})
   : frame_preserving_upd p x y
   = fun v -> f v
 
 (* A pcm_lens is a lens for a 'b inside an 'a such that upd lifts
    frame-preserving updates on 'b to frame-preserving updates on 'a *)
 noeq type pcm_lens (#a: Type u#a) (#b: Type u#b) (p: pcm a) (q: pcm b) = {
-  l: lens a b;
+  raw: lens a b;
   upd_resp_pcm:
     s: a -> v: b -> f:(b -> b) ->
     Lemma
-      (requires frame_preserv q f (l.get s) v)
-      (ensures frame_preserv p (upd l f) s (l.put v s));
+      (requires frame_pres q f (raw.get s) v)
+      (ensures frame_pres p (upd raw f) s (raw.put v s));
 }
 
 (* A ref is a pcm_lens combined with a Steel.Memory.ref for the base type 'a *)
 noeq type ref (#a: Type u#a) (#b: Type u#b) (p: pcm a) (q: pcm b) = {
   l: pcm_lens p q;
   r: M.ref a p;
+}
+
+let get_comp (l: lens 'a 'b) (m: lens 'b 'c) (s: 'a): 'c = m.get (l.get s)
+let put_comp (l: lens 'a 'b) (m: lens 'b 'c) (v: 'c) (s: 'a): 'a =
+  upd l (m.put v) s
+
+let lens_comp (l: lens 'a 'b) (m: lens 'b 'c): lens 'a 'c = {
+  get = get_comp l m;
+  put = put_comp l m;
+  get_put = (fun _ _ -> ());
+  put_get = (fun _ -> ());
+  put_put = (fun _ _ _ -> ());
+}
+
+// The following two lemmas aren't strictly necessary, but nice to verify
+open FStar.FunctionalExtensionality
+let upd_comp (l: lens 'a 'b) (m: lens 'b 'c) (f: 'c -> 'c) (s: 'a)
+  : Lemma (feq (upd (lens_comp l m) f) (upd l (upd m f)))
+  = ()
+let frame_pres_feq (p: pcm 'a) (f g: 'a -> 'a) (x y: 'a)
+  : Lemma (requires feq f g) (ensures frame_pres p f x y <==> frame_pres p g x y)
+  = ()
+
+let pcm_lens_comp (#p: pcm 'a) (#q: pcm 'b) (#r: pcm 'c)
+  (l: pcm_lens p q) (m: pcm_lens q r) : pcm_lens p r = {
+  raw = lens_comp l.raw m.raw;
+  upd_resp_pcm = (fun s v f ->
+    (* Goal:
+         s: a -> v: b -> f:(b -> b) ->
+         Lemma
+           (requires frame_pres q f ((comp l m).get s) v)
+           (ensures frame_pres p (upd (comp l m) f) s ((comp l m).put v s));
+       Since 
+         (feq (upd (comp l m) f) (upd l (upd m f))
+       and 
+         feq f g ==> frame_pres p f x y <==> frame_pres p g x y,
+       suff. to show
+         (ensures frame_pres p (upd l (upd m f)) s (l.put (m.put v (l.get s)) s)).
+       Because l respects pcms, suff. to show
+         (ensures frame_pres p (upd m f) (l.get s) (m.put v (l.get s))).
+       Because m respects pcms, suff. to show
+         (ensures frame_pres p f (m.get (l.get s)) v,
+       which we have by assumption
+         (requires frame_pres q f ((comp l m).get s) v). *)
+    m.upd_resp_pcm (l.raw.get s) v f;
+    l.upd_resp_pcm s (m.raw.put v (l.raw.get s)) (upd m.raw f)
+  );
 }
